fix two definitions and write two proofs

twophase/Twophase/Propositional.lean
@@ -15,7 +15,7 @@ import Twophase.Functional
 
 section
 -- The abstract type of resource managers.
-variable { RM : Type } [DecidableEq RM] [Hashable RM] [Repr RM]
+variable { RM : Type } [DecidableEq RM] [Hashable RM]
 
 -- The state `s` is the "current" state of the protocol.
 variable (s: ProtocolState RM)
@@ -27,6 +27,10 @@ def tm_rcv_prepared (rm: RM): Prop :=
     s.tmState = TMState.Init
   ∧ Message.Prepared rm ∈ s.msgs
   ∧ s'.tmPrepared = s.tmPrepared ∪ { rm }
+  ∧ s'.tmState = s.tmState
+  ∧ s'.rmState = s.rmState
+  ∧ s'.msgs = s.msgs
+  ∧ s'.all = s.all
 
 /-- The proposition version of `tmCommit`. -/
 def tm_commit: Prop :=
@@ -34,33 +38,62 @@ def tm_commit: Prop :=
   ∧ s.tmPrepared = s.all
   ∧ s'.tmState = TMState.Committed
   ∧ s'.msgs = s.msgs ∪ { Message.Commit }
+  ∧ s'.tmPrepared = s.tmPrepared
+  ∧ s'.rmState = s.rmState
+  ∧ s'.all = s.all
 
 /-- The proposition version of `tmAbort`. -/
 def tm_abort: Prop :=
     s.tmState = TMState.Init
   ∧ s'.tmState = TMState.Aborted
   ∧ s'.msgs = s.msgs ∪ { Message.Abort }
+  ∧ s'.tmPrepared = s.tmPrepared
+  ∧ s'.rmState = s.rmState
+  ∧ s'.all = s.all
 
 /-- The proposition version of `rmPrepare`. -/
 def rm_prepare (rm: RM): Prop :=
     s.rmState.get? rm = RMState.Working
   ∧ s'.rmState.get? rm = RMState.Prepared
+  ∧ ∀ rm' ∈ s.all, rm' ≠ rm →
+      s'.rmState.get? rm' = s.rmState.get? rm
   ∧ s'.msgs = s.msgs ∪ { Message.Prepared rm }
+  ∧ s'.tmState = s.tmState
+  ∧ s'.tmPrepared = s.tmPrepared
+  ∧ s'.all = s.all
 
 -- The proposition version of `rmChooseToAbort`. -/
 def rm_choose_to_abort (rm: RM): Prop :=
     s.rmState.get? rm = RMState.Working
   ∧ s'.rmState.get? rm = RMState.Aborted
+  ∧ ∀ rm' ∈ s.all, rm' ≠ rm →
+      s'.rmState.get? rm' = s.rmState.get? rm
+  ∧ s'.msgs = s.msgs
+  ∧ s'.tmState = s.tmState
+  ∧ s'.tmPrepared = s.tmPrepared
+  ∧ s'.all = s.all
 
 -- The proposition version of `rmRcvCommitMsg`. -/
 def rm_rcv_commit_msg (rm: RM): Prop :=
     Message.Commit ∈ s.msgs
   ∧ s'.rmState.get? rm = RMState.Committed
+  ∧ ∀ rm' ∈ s.all, rm' ≠ rm →
+      s'.rmState.get? rm' = s.rmState.get? rm
+  ∧ s'.msgs = s.msgs
+  ∧ s'.tmState = s.tmState
+  ∧ s'.tmPrepared = s.tmPrepared
+  ∧ s'.all = s.all
 
 -- The proposition version of `rmRcvAbortMsg`. -/
 def rm_rcv_abort_msg (rm: RM): Prop :=
     Message.Abort ∈ s.msgs
   ∧ s'.rmState.get? rm = RMState.Aborted
+  ∧ ∀ rm' ∈ s.all, rm' ≠ rm →
+      s'.rmState.get? rm' = s.rmState.get? rm
+  ∧ s'.msgs = s.msgs
+  ∧ s'.tmState = s.tmState
+  ∧ s'.tmPrepared = s.tmPrepared
+  ∧ s'.all = s.all
 
 -- Connecting the denotational and functional specifications.
 -- TODO: someone has to write the proofs :)
@@ -68,11 +101,51 @@ def rm_rcv_abort_msg (rm: RM): Prop :=
 theorem tm_rcv_prepared_correct (rm: RM):
   tm_rcv_prepared s s' rm ↔
     tmRcvPrepared RM s rm = some s' := by
-    sorry
+    apply Iff.intro
+    case mp =>
+      intro hrel
+      simp [tm_rcv_prepared] at hrel
+      rcases hrel with ⟨ h_tmState, h_msgs, h_tmPrepared', h_tmState', h_rmState', h_msgs', h_all' ⟩
+      simp [tmRcvPrepared]
+      simp [h_tmState]
+      simp [h_msgs]
+      rw [h_tmState] at h_tmState'
+      apply ProtocolState.ext
+      simp [h_all']; simp [h_tmPrepared']; simp [h_rmState']; simp [h_tmState'];
+      simp [h_tmPrepared']; simp [h_msgs']
+
+    case mpr =>
+      intro heq
+      simp [tmRcvPrepared] at heq
+      rcases heq with ⟨ ⟨ h_tmState, h_msgs ⟩, h_seq ⟩
+      unfold tm_rcv_prepared
+      simp [h_tmState, h_msgs]
+      rw [h_tmState] at h_seq
+      cases h_seq
+      simp
 
 theorem tm_commit_correct :
     tm_commit s s' ↔
-      tmCommit RM s = some s' := by sorry
+      tmCommit RM s = some s' := by
+      apply Iff.intro
+      case mp =>
+        intro hrel
+        simp [tm_commit] at hrel
+        rcases hrel with ⟨ h_tmState, h_tmPrepared, h_tmState', h_msgs', h_tmPrepared', h_rmState', h_all' ⟩
+        simp [tmCommit]
+        simp [h_tmState, h_tmPrepared]
+        apply ProtocolState.ext
+        simp [h_all']; simp [h_rmState']; simp [h_tmState'];
+        simp [h_tmPrepared']; simp [h_tmPrepared]; simp [h_msgs']
+
+      case mpr =>
+        intro heq
+        simp [tmCommit] at heq
+        rcases heq with ⟨ ⟨ h_tmState, h_tmPrepared ⟩, h_seq ⟩
+        unfold tm_commit
+        simp [h_tmState, h_tmPrepared]
+        cases h_seq
+        simp; simp [h_tmPrepared]
 
 theorem tm_abort_correct :
     tm_abort s s' ↔
